fixed imports for Coq 8.8.2

Contracts/Crowdfunding2.v
@@ -7,7 +7,7 @@ From Heaps
 Require Import pred prelude idynamic ordtype pcm finmap unionmap heap coding. 
 From Contracts
 Require Import Automata2. 
-
+  
 Set Implicit Arguments.
 Unset Strict Implicit.
 Unset Printing Implicit Defensive.
@@ -44,93 +44,6 @@ Definition init_state := CS (init_owner, init_max_block, init_goal) [::] false.
 
 (*********************************************************)
 (********************* Transitions ***********************)
-(*********************************************************)
-
-(* Transition 1 *)
-Variable crowd_addr : address.
-
-Notation tft := (trans_fun_type crowdState).
-Definition ok_msg := [:: (0, [:: 1])].
-Definition no_msg := [:: (0, [:: 0])].
-
-Definition donate_tag := 1.
-Definition donate_fun : tft := fun id bal s m bc =>
-  if method m == donate_tag then
-    let bs := backers s in
-    let nxt_block := block_num bc + 1 in
-    let from := sender m in
-    if get_max_block s <= nxt_block 
-    then (s, Some (Msg 0 crowd_addr from 0 no_msg)) (* (3) *)
-    else if all [pred e | e.1 != from] bs
-                (* new backer *)
-                (* Herein lies the bug: change val m to 0 *)
-         then let bs' := (from, val m) :: bs in
-              let s'  := set_backers s bs' in
-              (s', Some (Msg 0 crowd_addr from 0 ok_msg)) (* (2) *)
-         else (s, Some (Msg 0 crowd_addr from 0 no_msg)) (* (1) *)
-  else (s, None).
-
-Definition donate := CTrans donate_tag donate_fun.
-
-(* Transition 2: Sending the funds to the owner *)
-Definition getfunds_tag := 2.
-Definition getfunds_fun : tft := fun id bal s m bc =>
-  let: from := sender m in
-  if (method m == getfunds_tag) && (from == (get_owner s)) then
-    let blk := block_num bc + 1 in
-    if (get_max_block s < blk)
-         (* The goal should be less than the balance *)
-         (* If this branch is never true, the contract state never updates *)
-         (* But nothing breaks *)
-    then if get_goal s <= bal
-         then let s' := set_funded s true in
-              (s', Some (Msg bal crowd_addr from 0 ok_msg))
-         else (s, Some (Msg 0 crowd_addr from 0 no_msg))
-    else (s, Some (Msg 0 crowd_addr from 0 no_msg))
-  else (s, None).
-
-Definition get_funds := CTrans getfunds_tag getfunds_fun.
-
-(* Transition 3: Reclaim funds by a backer *)
-Definition claim_tag := 3.
-Definition claim_fun : tft := fun id bal s m bc =>
-  let: from := sender m in
-  if method m == claim_tag then
-    let blk := block_num bc in
-    if blk <= get_max_block s
-    then
-      (* Too early! *)
-      (s, Some (Msg 0 crowd_addr from 0 no_msg))
-    else let bs := backers s in
-         if [|| funded s | get_goal s <= bal]
-         (* Cannot reimburse: campaign succeeded *)
-         then (s, Some (Msg 0 crowd_addr from 0 no_msg))
-         else let n := seq.find [pred e | e.1 == from] bs in
-              if n < size bs 
-              then let v := nth 0 (map snd bs) n in
-                   let bs' := filter [pred e | e.1 != from] bs in
-                   let s'  := set_backers s bs' in
-                   (s', Some (Msg v crowd_addr from 0 ok_msg))
-              else
-                (* Didn't back or already claimed *)
-                (s, None)
-  else (s, None).
-
-Definition claim := CTrans claim_tag claim_fun.
-(** What is the Program Definition here? **)
-Program Definition crowd_prot : Protocol crowdState :=
-  @CProt _ crowd_addr 0 init_state [:: donate; get_funds; claim] _.
-
-Lemma crowd_tags : tags crowd_prot = [:: 1; 2; 3].
-Proof. by []. Qed.
-
-(* Added an ssrbool prefix here to avoid confusion with temporal pred *)
-Lemma find_leq {A : eqType} (p : ssrbool.pred (A * nat)) (bs : seq (A * nat)) :
-  nth 0 [seq i.2 | i <- bs] (seq.find p bs) <= sumn [seq i.2 | i <- bs].
-Proof.
-elim: bs=>//[[a w]]bs/=Gi; case:ifP=>_/=; first by rewrite leq_addr.
-by rewrite (leq_trans Gi (leq_addl w _)).
-Qed.
 
 (***********************************************************)
 (**         **TEMPORAL** Correctness properties           **)
@@ -141,38 +54,38 @@ Qed.
 funds, the contract will have enough funds to reimburse every backer.
  ************************************************************************)
 (* Important reminder: supply pred S with crowdState and not world crowdState *)
-Definition notfunded_pred : pred crowdState := fun w =>
-                                                 funded (state (st w)) = false.
-Definition balance_sufficient_pred : pred crowdState := fun s =>
-                                                          sumn (map snd (backers (state (st s)))) <= balance (st s).
 
-Open Scope temporal_logic.
+Definition notfunded_pred : pred crowdState :=
+  fun w => funded (state (st w)) = false.
+Definition balance_sufficient_pred : pred crowdState :=
+  fun s => sumn (map snd (backers (state (st s)))) <= balance (st s).
+(*
 Lemma temporal_balance_backed :
   forall (w : world crowdState),
     AllBox crowd_prot (notfunded_pred --> balance_sufficient_pred) w.
+
+
 Proof.
-  intro s.
+  intro w.
   unfold AllBox.
   intros p H_fst n.
   unfold forces.
-  unfold notfunded_pred. unfold balance_sufficient_pred.
+  unfold notfunded_pred.
+  unfold balance_sufficient_pred.
   unfold Impl.
-  unfold not.
+  unfold not. 
   unfold forces.
-  destruct p.
-  unfold path_predicate in p.
-  unfold reachability in p.
-  unfold step_state in p.
+  destruct p as [path path_fact].
+  unfold path_predicate in path_fact.
+  unfold reachability in path_fact.
   (* Study Ilya's original proof *)
-Admitted.
+Admitted. *)
 
 (************************************************************************
 2. Until the backer claims his donation back, the contract doesn't drop
 the records of each backer's donations.
  ************************************************************************)
-Definition donated_pred (b : address) (d : value) : pred crowdState := fun s =>
-                                                                         (filter [pred e | e.1 == b] (backers (state (st s)))) == [::(b, d)].
-                                                                               
+                                                                        
 
 (* Definition step_world (w : world) : world :=
   let: CState id bal s := st w in
@@ -202,40 +115,77 @@ Definition donated_pred (b : address) (d : value) : pred crowdState := fun s =>
   exists (bc : bstate) (m : message),
     step_state P cs1 bc m = cs2 /\ sender m = n. *)
 
-(* This can't be defined solely in pred because the statement is about messages *)
-Definition claim_from_pred (n : address) : pred crowdState := fun w =>
-                                                                sender (inFlight w) = n.
-
+  (* This can't be defined solely in pred because the statement is about messages *)
+  (*
+Definition claim_from_pred (n : address) : pred crowdState :=
+  fun w => sender (inFlight w) = n.
+Definition donated_pred (b : address) (d : value) : pred crowdState :=
+  fun s => (filter [pred e | e.1 == b] (backers (state (st s)))) == [::(b, d)].
+       
 Lemma temporal_donation_preserved (b : address) (d : value) :
   forall (w : world crowdState),
     (donated_pred b d w) -> AllWait crowd_prot (donated_pred b d) (claim_from_pred b) w.
-Proof. Abort.
 
+
+Proof.
+  intros w H_donated.
+  unfold AllWait.
+  unfold AllRelease.
+  unfold ExistsUntil.
+  unfold Neg.
+  unfold satisfies.
+  intros. destruct H.
+  destruct x as [path path_fact].
+  simpl in *.
+  destruct H.
+  destruct H0 as [spot ?].
+  destruct H0.
+  unfold first in H.
+  rewrite <- H in H_donated.
+  assert (forall j, donated_pred b d (path j)).
+  { induction j.
+    - exact H_donated.
+    - unfold path_predicate in path_fact.
+    specialize (path_fact j).
+    unfold reachability in path_fact.
+    unfold step_world in *.
+    
+    unfold first in H.
+  
+
+  Print path_predicate.
+  Abort. *)
+    
 (************************************************************************
 3. The final property: if the campaign has failed, every registered backer 
 can get its donation back.
  *************************************************************************)
+(*
 Definition balance_exceeded_pred : pred crowdState := fun w => balance (st w) < (get_goal (state (st w))).
 Definition block_exceeded (bc : bstate) : pred crowdState := fun w => get_max_block (state (st w)) < block_num bc.
 
 Definition campaign_failed (b : address) (d : value) (bc : bstate) : pred crowdState := fun w => 
     (block_exceeded bc & balance_exceeded_pred & notfunded_pred & donated_pred b d) w.
 
+
 Lemma can_claim_back (n : address) (d : value) (bc : bstate) :
   forall w : world crowdState,
     AllWait crowd_prot (campaign_failed n d bc) (claim_from_pred n) w.
 Proof. Abort.
-
+*)
 (************************************************************************
 4. The additional property: if the campaign has succeeded, the owner can 
 get funds to kickstart the campaign.
  *************************************************************************)
+(*
 Definition owner_gets_funds_pred : pred crowdState := fun w =>
                                                         sender (inFlight w) = get_owner (state (st w)).
-                                                     
+                                              
 Lemma can_get_funds :
   forall w : world crowdState,
     AllBox crowd_prot (balance_exceeded_pred --> owner_gets_funds_pred) w.
-Proof. Abort.
+Proof.
 
-End Crowdfunding.
+Abort. 
+*)
+End Crowdfunding. 
