Core/Automata2.v
@@ -1,15 +1,13 @@
 From mathcomp.ssreflect
-Require Import ssreflect ssrbool ssrnat eqtype ssrfun seq.
-From mathcomp Require Import path.
-Require Import Eqdep.
-From Heaps
-Require Import pred prelude idynamic ordtype pcm finmap unionmap heap coding.
+Require Import ssreflect ssrnat ssrfun ssrbool eqtype seq. 
+From VST.msl
+Require Import seplog Extensionality.
+(* Require Import ctl. *)
+
 Set Implicit Arguments.
 Unset Strict Implicit.
 Unset Printing Implicit Defensive.
 
-Ltac impl_e P P_implies_Q :=
-  apply P_implies_Q in P.
 Tactic Notation "spec" hyp(H) :=
   match type of H with ?a -> _ => 
     let H1 := fresh in (assert (H1: a); [|generalize (H H1); clear H H1; intro H]) end.
@@ -17,12 +15,7 @@ Tactic Notation "spec" hyp(H) constr(a) :=
   (generalize (H a); clear H; intro H). 
 Tactic Notation "spec" hyp(H) constr(a) constr(b) :=
   (generalize (H a b); clear H; intro H).
-Tactic Notation "spec" hyp(H) constr(a) constr(b) constr(c) :=
-  (generalize (H a b c); clear H; intro H).
-Tactic Notation "spec" hyp(H) constr(a) constr(b) constr(c) constr(d) :=
-  (generalize (H a b c d); clear H; intro H).
 
-(* A semantics of contracts with decidable deterministic transitions *)
 Section State.
 
 Definition value := nat.
@@ -36,7 +29,7 @@ Record message := Msg {
       sender : address;
       to     : address;
       method : tag;
-      body   :  payload
+      body   : payload
 }.
 
 (* Augmented state of a contract *)
@@ -54,34 +47,26 @@ Record bstate := BState {
 End State.
 
 Section Protocol.
-  
-Section Transitions.
+  Section Transitions.
 
-(* State type *)
-Variable S: Type.
+  (* A response from a transition *)
+  Definition resp_type := (address * value * tag * payload)%type.
+  Definition msg_bal (rt : resp_type) : value := rt.1.1.2.
 
-(* A response from a transition *)
-Definition resp_type := (address * value * tag * payload)%type.
-Definition msg_bal (rt : resp_type) : value := rt.1.1.2.
+  Variable (S : Type).
+  Definition trans_fun_type :=
+    address -> value -> S -> message -> bstate -> (S * option message).
+   Record ctransition :=
+    CTrans {
+        (* Unique tag of a transition in the protocol *)
+        ttag : tag;
+        (* Function (bstate, state, msg) :-> (state', option msg') *)
+        tfun : trans_fun_type;
+      }.
+   Definition idle_fun : trans_fun_type := fun _ _ s _ _ => (s, None).
+   Definition idle := CTrans 0 idle_fun. 
 
-(* Transitions are functions *)
-Definition trans_fun_type :=
-  address -> value -> S -> message -> bstate -> (S * option message).
-  
-(* Contract transition in the spirit of I/O automata *)
-Record ctransition :=
-  CTrans {
-      (* Unique tag of a transition in the protocol *)
-      ttag : tag;
-      
-      (* Function (bstate, state, msg) :-> (state', option msg') *)
-      tfun : trans_fun_type;
-  }.
-
-Definition idle_fun : trans_fun_type := fun _ _ s _ _ => (s, None).
-Definition idle := CTrans 0 idle_fun.
-
-End Transitions.
+  End Transitions.
 
 Record Protocol (S : Type) :=
   CProt {
@@ -96,15 +81,9 @@ Record Protocol (S : Type) :=
       (* All transitions have unique tags *)
       _ : uniq (map (@ttag _) transitions)
     }.
-
+                                 
 Definition tags {S : Type} (p : Protocol S) :=
   map (@ttag _) (transitions p).
-
-End Protocol.
-
-Section Semantics.
-
-Variables (S : Type) (p : Protocol S).
 
 (* Blockchain schedules *)
 Definition schedule := seq (bstate * message).
@@ -116,6 +95,8 @@ Fixpoint wf_sched (sch : schedule) :=
        all [pred s' | bnum <= block_num s'.1] sch' && wf_sched sch'
   else true.
 
+Variables (S : Type) (p : Protocol S).
+
 Definition step_state pre bc m : cstate S :=
   let: CState id bal s := pre in
   let: n := seq.find (fun t => ttag t == method m) (transitions p) in
@@ -126,140 +107,670 @@ Definition step_state pre bc m : cstate S :=
 
 Definition state0 := CState (acc p) (init_bal p) (init_state p).
 
-(*****************************************************)
-(*            Some modal connectives                 *)
-(*****************************************************)
-(* A temporal CTL semantics *)
-Record world :=
-  mkW {
-      inFlight : message;
-      st : cstate S;
-      b : bstate;
-      outFlight : option message
-    }.
-Parameter emptymsg : message.
-Parameter b0 : bstate.
-Definition world0 := mkW emptymsg state0 b0 None.
-Definition step_world (w : world) : world :=
-  let: CState id bal s := st w in
-  let: bc := b w in
-  let: m := inFlight w in
-  let: n := seq.find (fun t => ttag t == method m) (transitions p) in
-  let: tr := nth (idle S) (transitions p) n in
-  let: (s', out) := (tfun tr) id bal s m bc in
-  let: bal' := if out is Some m' then (bal + val m) - val m' else bal in
-  mkW m (CState id bal' s') bc out.
+Section Crowdfunding.
+
+Record crowdState := CS {
+   owner_mb_goal : address * nat * value;
+   backers : seq (address * value);
+   funded : bool;
+}.
+
+(* Administrative setters/getters *)
+Definition get_owner cs : address := (owner_mb_goal cs).1.1.
+Definition get_goal cs : value := (owner_mb_goal cs).2.
+Definition get_max_block cs : nat := (owner_mb_goal cs).1.2.
+
+Definition set_backers cs bs : crowdState :=
+  CS (owner_mb_goal cs) bs (funded cs).
+
+Definition set_funded cs f : crowdState :=
+  CS (owner_mb_goal cs) (backers cs) f.
+
+(* Parameters *)
+Variable init_owner : address.
+Variable init_max_block : nat.
+Variable init_goal : value.
+
+(* Initial state *)
+Definition init_crowdstate := CS (init_owner, init_max_block, init_goal) [::] false.
+
+(* Definition of the protocol *)
+Variable crowd_addr : address.
+
+Notation tft := (trans_fun_type crowdState).
+Definition ok_msg := [:: (0, [:: 1])].
+Definition no_msg := [:: (0, [:: 0])].
+
+Definition donate_tag := 1.
+Definition donate_fun : tft := fun id bal s m bc =>
+  if method m == donate_tag then
+    let bs := backers s in
+    let nxt_block := block_num bc + 1 in
+    let from := sender m in
+    if get_max_block s <= nxt_block
+    then (s, Some (Msg 0 crowd_addr from 0 no_msg))
+    else if all [pred e | e.1 != from] bs
+         (* new backer *)
+         then let bs' := (from, val m) :: bs in
+              let s'  := set_backers s bs' in
+              (s', Some (Msg 0 crowd_addr from 0 ok_msg))
+         else (s, Some (Msg 0 crowd_addr from 0 no_msg))
+  else (s, None).
+
+Definition donate := CTrans donate_tag donate_fun.
+
+Definition getfunds_tag := 2.
+Definition getfunds_fun : tft := fun id bal s m bc =>
+  let: from := sender m in
+  if (method m == getfunds_tag) && (from == (get_owner s)) then
+    let blk := block_num bc + 1 in
+    if (get_max_block s < blk)
+    then if get_goal s <= bal
+         then let s' := set_funded s true in
+              (s', Some (Msg bal crowd_addr from 0 ok_msg))
+         else (s, Some (Msg 0 crowd_addr from 0 no_msg))
+    else (s, Some (Msg 0 crowd_addr from 0 no_msg))
+  else (s, None).
+
+Definition get_funds := CTrans getfunds_tag getfunds_fun.
+
+Definition claim_tag := 3.
+Definition claim_fun : tft := fun id bal s m bc =>
+  let: from := sender m in
+  if method m == claim_tag then
+    let blk := block_num bc in
+    if blk <= get_max_block s
+    then
+      (* Too early! *)
+      (s, Some (Msg 0 crowd_addr from 0 no_msg))
+    else let bs := backers s in
+         if [|| funded s | get_goal s <= bal]
+         (* Cannot reimburse: campaign suceeded *)
+         then (s, Some (Msg 0 crowd_addr from 0 no_msg))
+         else let n := seq.find [pred e | e.1 == from] bs in
+              if n < size bs
+              then let v := nth 0 (map snd bs) n in
+                   let bs' := filter [pred e | e.1 != from] bs in
+                   let s'  := set_backers s bs' in
+                   (s', Some (Msg v crowd_addr from 0 ok_msg))
+              else
+                (* Didn't back or already claimed *)
+                (s, None)
+  else (s, None).
+
+Definition claim := CTrans claim_tag claim_fun.
+
+Program Definition crowd_prot : Protocol crowdState :=
+  @CProt _ crowd_addr 0 init_crowdstate [:: donate; get_funds; claim] _.
+
+Lemma crowd_tags : tags crowd_prot = [:: 1; 2; 3].
+Proof. by []. Qed.
+
+(* 
+Lemma find_leq {T : eqType} (p : pred (T * nat)) (bs : seq (T * nat)) :
+  nth 0 [seq i.2 | i <- bs] (seq.find p bs) <= sumn [seq i.2 | i <- bs].
+Proof.
+elim: bs=>//[[a w]]bs/=Gi; case:ifP=>_/=; first by rewrite leq_addr.
+by rewrite (leq_trans Gi (leq_addl w _)).
+Qed.
+ *)
+
+End Crowdfunding.
+
+End Protocol.
+
+
+Section World.
+(* World type *)
+  Variables (T : Type) (prot : Protocol T).
+ 
+  Record world T := mkW
+      {
+        inFlight : message;
+        st : cstate T;
+        b : bstate;
+        outFlight : option message
+      }.
+
+    Parameter emptymsg: message.
+    Parameter b0 : bstate.
+    Definition world0 := mkW emptymsg (state0 prot) b0 None. (* First world *)
+    Definition step_world (w : world T) : world T :=
+     let: CState id bal s := st w in
+     let: bc := b w in
+     let: m := inFlight w in
+     let: n := seq.find (fun t => ttag t == method m) (transitions prot) in
+     let: tr := nth (idle T) (transitions prot) n in
+     let: (s', out) := (tfun tr) id bal s m bc in
+     let: bal' := if out is Some m' then (bal + val m) - val m' else bal in
+     mkW m (CState id bal' s') bc out.
   
-Definition pred := world -> Prop.
-(*
-Definition reachability : cstate S -> cstate S -> Prop := fun s1 s2 =>
-                                                          exists (bc : bstate) (m : message),
-                                                            step_state s1 bc m = s2. *)
+    Definition pred := world T -> Prop.
+  
+    Definition reachability : world T -> world T -> Prop :=
+    fun w1 w2 => step_world w1 = w2.
 
-Definition reachability : world -> world  -> Prop := fun w1 w2 => step_world w1 = w2.
-Definition path := nat -> world.
-Definition first (p : path) : world := p 0. 
+    Lemma reachability_trans :
+      forall (w1 w2 w3 : world T),
+        reachability w1 w2 -> reachability w2 w3 -> reachability w1 w3.
+    Proof. Abort. (* This is the exactly not what we want *)
 
-(* A good path is a path that begins with the initial state and satisfies the reachability relation *)
-Definition path_predicate (p : path) := (* p 0 = state0 /\ *) forall n, reachability (p n) (p (n + 1)).
-Definition gpath : Type := {p : path & path_predicate p }.
-Definition gpath_proj1 : gpath -> (nat -> world) := fun gp =>  match gp with | existT a _ => a end.
-Coercion gpath_proj1 : gpath >-> Funclass.
+    (* Path definitions *)
+    Definition path := nat -> world T.
+    Definition first (p : path) : world T := p 0.
+    Definition path_predicate (p : path) := forall n, reachability (p n) (p (n.+1)).
+    (** Contention : paths can't all start with world0 **) 
+    (* Good path sigma-type definitions *)
+    Definition gpath : Type := {p : path & path_predicate p}.
+    (* Projection functions for sigma type good paths *)
+    Definition gpath_proj1 : gpath -> (nat -> world T) := fun gp => 
+        match gp with
+        | existT a _ => a
+        end.
+    Coercion gpath_proj1 : gpath >-> Funclass. 
+    Definition gpath_proj2 (gp : gpath) : (path_predicate (gpath_proj1 gp)) :=
+        match gp with
+        | existT _ b => b
+        end.    
 
-(* State satisfaction *)
-Definition forces (s : world) (p : pred) : Prop :=
-  p s.
-Notation "w '|=' P" := (forces w P) (at level 80, no associativity).
+    (* A cacophany of path constructions *)
+    (* Constructing a random path *) 
+    Fixpoint step_n_times (w : world T) (n : nat) :=
+      match n with
+      | 0 => w
+      | S n' => step_world (step_n_times w n')
+      end.
+    
+    Definition make_path (w : world T) : path := step_n_times w.
 
-(* Stuff in Prop *)
+    Lemma rewrite_step_world_S :
+      forall (n : nat) (w : world T),
+        step_n_times w (n.+1) = step_world (step_n_times w n).
+      Proof. reflexivity. Qed.
+
+    Lemma step_world_swap_helper :
+      forall (n : nat) (w : world T),
+        step_world (step_n_times w n) =
+        step_n_times (step_world w) n.
+    Proof.
+      intros n w.
+      induction n.
+      - reflexivity.
+      - rewrite rewrite_step_world_S.
+        rewrite IHn.
+        rewrite rewrite_step_world_S.
+        reflexivity.
+    Qed.
+
+    Lemma step_world_swap :
+      forall n : nat,
+        step_world (step_n_times (step_world world0) n) =
+        step_n_times (step_world (step_world world0)) n.
+    Proof.
+      induction n.
+      - reflexivity.
+      - rewrite step_world_swap_helper.
+        reflexivity.
+    Qed.
+    
+    Lemma step_world_ind :
+      forall n : nat,
+        step_world (step_n_times world0 n) = step_n_times world0 n.+1.
+    Proof.
+      induction n.
+      - simpl; reflexivity.
+      - simpl. reflexivity.
+    Qed.
+
+    Lemma about_p : path_predicate (make_path world0).
+    Proof.
+      unfold path_predicate.
+      induction n.
+      - simpl. unfold reachability. reflexivity.
+      - unfold reachability in *.
+        unfold make_path in *.
+        rewrite <- IHn.
+        simpl. reflexivity.
+    Qed.
+
+    Lemma about_p_hole :
+      forall w : world T,
+        path_predicate (make_path w).
+    Proof.
+      unfold path_predicate.
+      induction n.
+      - simpl. unfold reachability. reflexivity.
+      - unfold reachability in *.
+        unfold make_path in *.
+        rewrite <- IHn.
+        simpl. reflexivity.
+    Qed.
+
+    Definition gp : gpath := (existT _ (make_path world0) about_p).
+    (* Can you make a sigma type with a dependent type? *)
+    Parameter generic_world : world T.
+    Check (about_p_hole generic_world).
+    Definition gp_hole (w : world T) : gpath := (existT _ (make_path w) (about_p_hole w)).
+    (* The answer is yes *)
+
+    (* Constructing an offset path *)
+    Definition make_offset_path (p : path) : path := fun n => p n.+1.
+    Definition make_offset_path' (gp : gpath) : path := fun n => gpath_proj1 gp n.+1.
+    Lemma about_offset_path :
+      forall p : path,
+        path_predicate p ->
+        path_predicate (make_offset_path p).
+    Proof.
+      intros p H_p.
+      unfold make_offset_path.
+      unfold path_predicate in *.
+      intro n. 
+      exact (H_p n.+1).
+    Qed.
+    Lemma about_offset_path' :
+      forall gp : gpath,
+        path_predicate (make_offset_path' gp). 
+    Proof.
+      intro gp.
+      destruct gp. unfold path_predicate in p.
+      unfold make_offset_path'.
+      unfold gpath_proj1.
+      unfold path_predicate.
+      intros n.
+      exact (p n.+1).
+    Qed.
+    Definition gp_offset (p : path) (pred : path_predicate p) : gpath :=
+      (existT _ (make_offset_path p) (about_offset_path pred)).
+    Definition gp_offset' (gp : gpath) : gpath :=
+      (existT _ (make_offset_path' gp) (about_offset_path' gp)).
+
+    (* Constructing a backwards offset path *)
+    Definition make_backwards_offset_path (w0 : world T) (p : path) : path :=
+      fun n => if eqn n 0 then w0 else (p n.-1).
+    Definition make_backwards_offset_path' (w0 : world T) (gp : gpath) : path :=
+      fun n => if eqn n 0 then w0 else gpath_proj1 gp n.-1.
+    Lemma about_backwards_offset_path :
+      forall (p : path) (w0 : world T),
+        path_predicate p ->
+        reachability w0 (p 0) -> 
+        path_predicate (make_backwards_offset_path w0 p).
+    Proof.
+      intros p w0 H_p.
+      unfold make_backwards_offset_path.
+      unfold path_predicate in *.
+      destruct n.
+      simpl. exact H.
+      simpl. apply (H_p n).
+    Qed.
+    Lemma about_backwards_offset_path' :
+      forall (gp : gpath) (w0 : world T),
+        reachability w0 (gpath_proj1 gp 0) -> 
+        path_predicate (make_backwards_offset_path' w0 gp). 
+    Proof.
+      intros gp w0 H_0.
+      destruct gp. unfold path_predicate in p.
+      unfold make_backwards_offset_path'.
+      unfold gpath_proj1.
+      unfold path_predicate.
+      destruct n.
+      simpl. exact H_0.
+      simpl. apply (p n).
+    Qed.
+    Definition gp_backwards_offset
+               (w0 : world T) (p : path)
+               (pred : path_predicate p)
+               (r : reachability w0 (p 0)) : gpath :=
+      (existT _ (make_backwards_offset_path w0 p) (about_backwards_offset_path pred r)).
+    Definition gp_backwards_offset'
+               (w0 : world T) (gp : gpath)
+               (r : reachability w0 (gpath_proj1 gp 0)) : gpath :=
+      (existT _ (make_backwards_offset_path' w0 gp) (about_backwards_offset_path' r)).    
+
+    (* Satisfaction definition *)
+    Definition satisfies (w : world T) (p : pred) : Prop := p w.
+    (* I'm not sure that the following metalogic entail is necessary *)
+    Definition entails (p q : pred) : Prop :=
+      forall w, (satisfies w p) -> (satisfies w q).
+    Definition equiv (p q : pred) : Prop := entails p q /\ entails q p.
+    
+  End World. 
+
 Axiom LEM : forall P : Prop, P \/ ~ P.
-Definition entails P Q : Prop :=
-  forall w,  (w |= P) -> (w |= Q).
-Definition equiv P Q : Prop :=
-  entails P Q /\ entails Q P.
+Notation "w '|=' p" := (satisfies w p) (at level 80, no associativity).
 
-(* Stuff in pred *)
-Parameter Top : pred.
-Parameter Bottom : pred.
-Definition Neg P : pred := fun w =>
-                             ~(w |= P).
-Definition Conj P Q : pred := fun w =>
-                                (w |= P) /\ (w |= Q).
-Definition Disj P Q : pred := fun w =>
-                                (w |= P) \/ (w |= Q).
-Definition Impl P Q : pred := fun w =>
-                                ~(w |= P) \/ (w |= Q).
+Section CTL.
+  Variables (S : Type) (prot : Protocol S).  
+Local Open Scope logic.
 
+(* NatDed in Prop  *) 
+Instance natded_prop : NatDed Prop :=
+  { andp p q := p /\ q;
+    orp p q := p \/ q;
+    exp t p := exists t, p t;
+    allp t p := forall t, p t;
+    imp p q := p -> q;
+    prop p := p;
+    derives p q := p -> q;
+  }.
+- intros. apply prop_ext. split. exact H. exact H0.
+- intros. apply H.
+- intros. apply H0; apply H. exact H1.
+- intros. split.  apply H; exact H1. apply H0; exact H1. 
+- intros. destruct H0. apply H; exact H0.
+- intros. apply H. destruct H0. exact H1. 
+- intros. destruct H1. apply H; exact H1. apply H0; exact H1.
+- intros. left. apply H; exact H0.
+- intros. right. apply H. exact H0. 
+- intros. exists x. apply H. exact H0. 
+- intros. destruct H0. apply (H x). exact H0. 
+- intros. apply H.  exact (H0 x).
+- intros. apply (H t). exact H0. 
+- intros. split. intros. apply H. split. apply H0. apply H1.
+- intros. apply H. destruct H0. exact H0. destruct H0.  exact H1. 
+- intros. apply H. exact H0. trivial. 
+- intros. exact H.
+- intros. apply H; exact H0.
+- intros. exact (H b1).
+Defined.
 
-(* Temporal operator definitions *)
-Definition AllNext (P : pred) : pred := fun w =>  
-  forall p : gpath, first p = w ->
-            p 1 |= P.
-Definition ExistsNext (P : pred) : pred := fun w =>  
-  exists p : gpath, first p = w ->
-            p 1 |= P.
-Definition AllBox P : pred := fun w =>  
-  forall p : gpath, first p = w ->
-            forall n, p n |= P.
-Definition ExistsBox P : pred := fun w =>  
-  exists p : gpath, first p = w ->
-            forall n, p n |= P.
-Definition AllFuture P : pred := fun w =>  
-  forall p : gpath, first p = w ->
-            exists n, p n |= P.
-Definition ExistsFuture P : pred := fun w =>  
-  exists p : gpath, first p = w ->
-            exists n, p n |= P.
-Definition AllUntil P Q : pred := fun w =>  
-  forall p : gpath, first p = w ->
-            exists n, p n |= Q /\
-                      forall m, m < n -> p m |= P.
-Definition ExistsUntil P Q : pred := fun w =>  
-  exists p : gpath, first p = w ->
-            exists n, p n |= Q /\
-                      forall m, m < n -> p m |= P.
+(* NatDed in pred *)
+Instance natded_pred (S : Type) : NatDed (pred S) :=
+  {
+    andp p q := fun w => (w |= p) /\ (w |= q);
+    orp p q := fun w => (w |= p) \/ (w |= q);
+    exp t p := fun w => exists n, (w |= p n);
+    allp t p := fun w => forall n, (w |= p n);
+    imp p q := fun w => (w |= p) -> (w |= q);
+    prop p := fun w => p;
+    derives p q := forall w, (w |= p) -> (w |= q);
+  }.
 
-Delimit Scope temporal_logic with temporal_logic.
-Open Scope temporal_logic.
+- intros.
+  apply extensionality. intros x.
+  apply prop_ext. split.
+  apply H. apply H0.
+- intros; trivial.
+- intros. apply H0. apply H. exact H1.
+- intros. split. 
+  assert (H_copy := H1).
+  apply H in H1. exact H1.
+  apply H0 in H1. exact H1. 
+- intros. apply H. unfold satisfies in H0.
+  destruct H0. exact H0. 
+- intros. apply H. apply H0.
+- intros. unfold satisfies in H1. destruct H1.
+  apply H in H1. exact H1. apply H0 in H1. exact H1.
+- intros. apply H in H0. unfold satisfies in *. left. exact H0.
+- intros. unfold satisfies in *. right. apply H. exact H0.
+- intros. unfold satisfies in *. spec H w. exists x. apply H. exact H0. 
+- intros. unfold satisfies in *. destruct H0. spec H x. apply H. exact H0.
+- intros. apply H.  unfold satisfies in *. spec H0 x. exact H0.
+- intros. unfold satisfies in *. intro n. spec H n w. apply H. exact H0.
+- intros. split. intros. unfold satisfies in *.
+  assert (Q w \/ ~ Q w). apply LEM. destruct H1. intro. apply H. split. exact H0.
+  exact H1. intro. contradiction.
+- intros. unfold satisfies in *. apply H; auto.
+- intros. unfold satisfies in *. destruct H0. exact H0. destruct H0. exact H1. 
+- intros. unfold satisfies in *. apply H. exact H0. auto. 
+- intros. unfold satisfies in *. exact H.
+- intros. apply H.
+- intros. apply H.
+Defined.
 
-Notation "P <=> Q" := (equiv P Q) (at level 35, no associativity).
-Notation "~~ P" := (Neg P) : temporal_logic.
-Notation "P & Q" := (Conj P Q) (at level 65, left associativity) : temporal_logic.
-Notation "P || Q" := (Disj P Q) : temporal_logic.
-Notation "P --> Q" := (Impl P Q) (at level 35, no associativity) : temporal_logic.
-Notation "'A' '[' P 'U' Q ']'" := (AllUntil P Q) (at level 35, no associativity) : temporal_logic.
-Notation "'E' '[' P 'U' Q ']'" := (ExistsUntil P Q) (at level 35, no associativity) : temporal_logic.
+(* CTL class *)
+Class CTL (T : Type) {ND: NatDed T} : Type := mkCTL {
+  all_next : T -> T ;
+  exists_next : T -> T ;
+  all_future : T -> T ;
+  exists_future : T -> T;
+  all_box : T -> T;
+  exists_box : T -> T;
+  all_until : T -> T -> T;
+  exists_until : T -> T -> T;  
+  ctl_1 : forall (P : T), all_box P |-- (P && all_next (all_box P));
+  ctl_2 : forall (P : T), (P && all_next (all_box P)) |-- all_box P;
+  ctl_3 : forall (P : T), exists_box P |-- (P && (exists_next (exists_box P)));
+  ctl_4 : forall (P : T), (P && exists_next (exists_box P)) |-- exists_box P;
+  (* The following equivalences suffice to prove the adequate connectives result *)
+  equiv_1 : forall (P : T), all_next P |-- (exists_next (P --> FF) --> FF);
+  equiv_2 : forall (P : T), all_future P |-- (exists_box (P --> FF) --> FF);
+  equiv_3 : forall (P : T), all_box P |-- (exists_future (P --> FF) --> FF);
+  equiv_4 : forall (P : T), all_future P |-- all_until TT P;
+  equiv_5 : forall (P : T), exists_future P |-- exists_until TT P;
+  equiv_6 : forall (P Q : T), all_until P Q |-- (exists_until (P --> FF)
+                                                              ((P --> FF) && (Q --> FF))
+                                                              --> FF) && all_future Q; 
+                                                }.
 
-(* Temporal operator extensions *)
-Definition AllRelease P Q : pred := 
-  ~~ (ExistsUntil (~~ P) (~~ Q)).
-Definition ExistsRelease P Q : pred :=
-  ~~ (AllUntil (~~ P) (~~ Q)).
-Definition AllWait P Q : pred :=
-  AllRelease P (P || Q).
-Definition ExistsWait P Q : pred :=
-  ExistsRelease P (P || Q).
+Instance lift_ctl_modal : (@CTL _ (natded_pred S)) :=
+  { all_next p := fun w =>
+                    forall gp : gpath prot,
+                      first gp = w -> gp 1 |= p;
+    exists_next p := fun w =>
+                       exists gp : gpath prot,
+                         first gp = w /\ gp 1 |= p;
+    all_future p := fun w =>
+                      forall gp : gpath prot,
+                        first gp = w -> exists n, gp n |= p;
+    exists_future p := fun w =>
+                         forall gp : gpath prot,
+                           first gp = w -> exists n, gp n |= p;
+    all_box p := fun w =>
+                   forall gp : gpath prot,
+                     first gp = w -> forall n, gp n |= p;
+    exists_box p := fun w =>
+                      exists gp : gpath prot,
+                        first gp = w /\ forall n, gp n |= p;
+    all_until p q := fun w =>
+                       forall gp : gpath prot,
+                         first gp = w ->
+                         exists n, gp n |= q
+                                   /\ forall m, m < n -> gp m |= p;
+    exists_until p q := fun w =>
+                          exists gp : gpath prot,
+                            first gp = w
+                            /\ exists n, gp n |= q
+                                         /\ forall m, m < n -> gp m |= p;
+  }.
+(* Proving ctl_1 : forall (P : T), all_box P |-- (P && all_next (all_box P)) *)
+intros P.
+unfold derives. simpl. unfold satisfies in *. 
+intros w H_AG.
+split.
+spec H_AG (gp_hole prot w).
+unfold first in H_AG.
+assert ((gp_hole prot w) 0 = w).
+simpl. reflexivity.
+exact (H_AG H 0).
+intros gp H_first gp' H_first' n.
+assert (exists m, gp m = gp' n).
+exists n.+1.
+unfold gpath in gp, gp'.
+destruct gp, gp'.
+unfold path_predicate in p, p0.
+simpl in H_first'.
+unfold first in H_first'.
+simpl in H_first, H_first'. simpl.
+assert (p_copy := p).
+assert (p0_copy := p0).
+unfold reachability in p, p0.
+induction n.
+symmetry; exact H_first'.
+rewrite <- (p n.+1).
+rewrite <- (p0 n). rewrite <- IHn. 
+reflexivity.
+destruct H.
+rewrite <- H. 
+spec H_AG gp.
+apply H_AG. exact H_first.
+(* Proving ctl_2 : forall (P : T), (P && all_next (all_box P)) |-- all_box P *)
+intros P.
+unfold derives. simpl. unfold derives in *.
+intros w H gp H_first n. unfold satisfies in *.
+destruct H as [H_P H_AXAG].
+spec H_AXAG gp.
+(* The following series of bookkeeping moves is annoying but necessary to 
+circumvent the high demands of automation from apply tactic *)
+assert (forall gp' : gpath prot, first gp' = gp 1 -> forall n : nat, P (gp' n)).
+apply H_AXAG; exact H_first.
+clear H_AXAG.
+rename H into H_AXAG.
+spec H_AXAG (gp_offset' gp).
+simpl in H_AXAG.
+assert (first (make_offset_path' gp) = gp 1).
+unfold make_offset_path'.
+unfold first. reflexivity.
+(* Another series of redundant bookkeeping moves *)
+assert (forall n : nat, P (make_offset_path' gp n)).
+apply H_AXAG; exact H.
+clear H_AXAG H.
+unfold make_offset_path' in H0.
+case n.
+unfold first in H_first; rewrite H_first; exact H_P. 
+exact H0.
+(* Proving ctl_3 : forall (P : T), exists_box P |-- (P && (exists_next (exists_box P))) *)
+intros P.
+unfold derives. simpl. unfold satisfies in *. 
+intros w H_EG.
+split.
+destruct H_EG. destruct H. 
+spec H0 0.
+unfold first in H; rewrite H in H0; exact H0.
+destruct H_EG. destruct H.
+exists x. split.
+exact H. exists (gp_offset' x).
+split.
+simpl. unfold make_offset_path'. unfold first. reflexivity.
+intro n.
+spec H0 n.+1.
+unfold gp_offset'.
+unfold make_offset_path'. simpl.
+exact H0.
+(* Proving ctl_4 : forall (P : T), (P && (exists_next (exists_box P))) |-- exists_box P *)
+intro P.
+unfold derives. simpl. unfold satisfies in *.
+intros. destruct H.
+repeat destruct H0.
+destruct H1. destruct H0.
+assert (reachability prot (x 0) (x 1)).
+unfold gpath in x. 
+destruct x.
+unfold path_predicate in p.
+simpl.
+exact (p 0).
+assert (reachability prot (x 0) (x0 0)).
+unfold first in H0; rewrite H0; exact H2.
+clear H2.
+exists (gp_backwards_offset' H3).
+split.
+simpl. unfold make_backwards_offset_path'.
+unfold first. reflexivity.
+unfold gp_backwards_offset'.
+destruct n.
+simpl. exact H.
+simpl.
+unfold make_backwards_offset_path'.
+simpl. exact (H1 n).
+(* Proving equiv_1 : AX P == ~ EX (~P) *)
+intro P.
+unfold derives. simpl. unfold satisfies in *.
+intros w H_1 H.
+repeat destruct H.
+spec H_1 x.
+assert (first x = first x) by reflexivity.
+apply H_1 in H.
+apply H0.
+exact H.
+(* Proving equiv_2 : AF P == ~ EG (~P) *)
+intro P. 
+unfold derives. simpl. unfold satisfies in *.
+intros w H_AG H_EG.
+destruct H_EG.
+destruct H.
+spec H_AG x.
+apply H_AG in H.
+destruct H.
+spec H0 x0.
+apply H0. exact H.
+(* Proving equiv_3 : AG p == ~ EF (~P) *)
+intro P. 
+unfold derives. simpl. unfold satisfies in *.
+intros w H_AG H_EF.
+spec H_AG (gp_hole prot w).
+assert (first (gp_hole prot w) = w).
+unfold first. unfold gp_hole. simpl; reflexivity.
+assert (forall n : nat, P ((gp_hole prot w) n)).
+apply H_AG. exact H.
+clear H_AG.
+spec H_EF (gp_hole prot w).
+assert (exists n : nat, P ((gp_hole prot w) n) -> False).
+apply H_EF; exact H.
+destruct H1.
+apply H1.
+spec H0 x. exact H0.
+(* Proving equiv_4 : AF P == A[T U P] *)
+intro P. 
+unfold derives. simpl. unfold satisfies in *.
+intros w H_AF gp H_first.
+spec H_AF gp.
+assert (exists n : nat, P (gp n)).
+apply H_AF.
+exact H_first.
+destruct H. exists x. split. exact H.
+intros. reflexivity.
+(* Proving equiv_5 : EF P == E[T U P] *)
+intro P.
+unfold derives. simpl. unfold satisfies in *.
+intros w H_EF.
+spec H_EF (gp_hole prot w).
+assert (first (gp_hole prot w) = w) by reflexivity.
+apply H_EF in H.
+clear H_EF.
+destruct H. 
+exists (gp_hole prot w).
+split.
+reflexivity.
+exists x. 
+split.
+exact H.
+intros; reflexivity.
+(* Proving ind : P -> AN P == AG P 
+intro P.
+unfold derives. simpl. unfold satisfies in *.
+intros w H_AN gp H_first n.
+induction n.
+unfold first in H_first; rewrite H_first.
+apply H_AN.
+intros gp' H_first'.
+ This seems unprovable *)
+(* Proving equiv_6 : A[P U Q] == ~E[~P U (~P /\ ~Q)] /\ (AF Q) *)
+intros P Q. 
+unfold derives. simpl. unfold satisfies in *.
+intros w H_AU.
+split.
+intros H_EU.
+destruct H_EU.
+repeat destruct H.
+destruct H0. repeat destruct H.
+spec H_AU x.
+assert (first x = first x) by reflexivity. 
+apply H_AU in H.
+clear H_AU.
+(* Clearly this needs to be proven via contradiction *)
+rename H into H_EU. rename x into gp.
+destruct H_EU.
+destruct H.
+assert (x < x0 \/ ~ x < x0).
+apply LEM.
+destruct H3.
+spec H0 x. 
+apply H0 in H3.
+inversion H3.
+Abort.
 
-Notation "'A' '[' P 'W' Q ']'" := (AllWait P Q) (at level 35, no associativity) : temporal_logic.
-Notation "'E' '[' P 'W' Q ']'" := (ExistsWait P Q) (at level 35, no associativity) : temporal_logic.
+End CTL.
 
-End Semantics.
-
-Delimit Scope temporal_logic with temporal_logic.
-
-Notation "P <=> Q" := (equiv P Q) (at level 35, no associativity).
-Notation "~~ P" := (Neg P) : temporal_logic.
-Notation "P & Q" := (Conj P Q) (at level 65, left associativity) : temporal_logic.
-Notation "P || Q" := (Disj P Q) : temporal_logic.
-Notation "P --> Q" := (Impl P Q) (at level 35, no associativity) : temporal_logic.
-
-(* Given the sigma-type gpath, we can safely say this
-because gpath will handle the proof of reachability *)
-Definition reachable (S : Type) (P : Protocol S) (st st' : world S) :=
-  exists (p : gpath P),
-  exists (n m : nat),
-    p n = st /\ p m = st.
-
+(* Next we need to deal with the notions of induction and safety *) 
 (* A stronger safety property *)
 Definition safe  (S : Type) (P : Protocol S) (pr : pred S) (pth : gpath P) :=
   forall n : nat, pr (pth n).
@@ -276,4 +787,5 @@ Proof.
   induction n.
   exact m.
   apply H. exact IHn.
-Qed. 
+Qed.
+
